

Suppose an experiment has sample space  $S = \{a, b, c, d, e, f, g, h\}$  with equiprobable outcomes. How many events in  $S$  occur when the experiment is conducted once?

- (a) 128
- (b) 1
- (c) 256
- (d) 2
- (e)  $\binom{8}{2}$
- (f)  $\binom{8}{1}\binom{8}{7}$
- (g) 0
- (h) 8
- (i) 7
- (j) None of these

**Solution:**  $2^7 = 128$ .

Suppose an experiment has sample space  $S = \{a, b, c, d, e, f, g, h\}$  with equiprobable outcomes. Define the following three events:

$$R = \{a, b, c, d, e\}$$

$$T = S - \{e, h\}$$

$$Q = \{d, g, h\}.$$

Which of the following events is independent of the event  $RT$  ?

- (a)  $TQ$
- (b)  $\{a, c\}$
- (c)  $Q^c R^c$
- (d)  $R^c Q$
- (e)  $\{a, b, c\}$
- (f)  $\{a, b\}$
- (g)  $T^c$
- (h)  $\{a\}$
- (i)  $R^c$
- (j) None of these

Suppose an experiment has sample space  $S = \{a, b, c, d, e, f, g, h\}$  with equiprobable outcomes. Define the following three events:

$$T = \{a, b, c, d, e\}$$

$$R = S - \{e, h\}$$

$$Q = \{d, g, h\}.$$

Which of the following events is independent of the event  $TR$  ?

- (a)  $RQ$
- (b)  $\{a, c\}$
- (c)  $Q^c T^c$
- (d)  $T^c Q$
- (e)  $\{a, b, c\}$
- (f)  $\{a, b\}$
- (g)  $R^c$
- (h)  $\{a\}$
- (i)  $T^c$
- (j) None of these

Suppose an experiment has sample space  $S = \{a, b, c, d, e, f, g, h\}$  with equiprobable outcomes. Define the following three events:

$$R = \{a, b, c, d, e\}$$

$$Q = S - \{e, h\}$$

$$T = \{d, g, h\}.$$

Which of the following events is independent of the event  $RQ$  ?

- (a)  $QT$
- (b)  $\{a, c\}$
- (c)  $T^c R^c$
- (d)  $R^c T$
- (e)  $\{a, b, c\}$
- (f)  $\{a, b\}$
- (g)  $Q^c$
- (h)  $\{a\}$
- (i)  $R^c$
- (j) None of these

Suppose an experiment has sample space  $S = \{a, b, c, d, e, f, g, h\}$  with equiprobable outcomes. Define the following three events:

$$T = \{a, b, c, d, e\}$$

$$Q = S - \{e, h\}$$

$$R = \{d, g, h\}.$$

Which of the following events is independent of the event  $TQ$  ?

- (a)  $QR$
- (b)  $\{a, c\}$
- (c)  $R^c T^c$
- (d)  $T^c R$
- (e)  $\{a, b, c\}$
- (f)  $\{a, b\}$
- (g)  $Q^c$
- (h)  $\{a\}$
- (i)  $T^c$
- (j) None of these

**Solution:** Let

$$Q = \{a, b, c, d, e\}$$

$$R = S - \{e, h\}$$

$$T = \{d, g, h\}.$$

Then,  $P(QR) = P(\{a, b, c, d\}) = 1/2$  and  $P(QR|RT) = P(QRT)/P(RT) = P(\{d\})/P(\{d, g\}) = 1/2 = P(QR)$ , so  $QR$  is independent of  $RT$ . All the other answers are nonempty and either subsets of, or disjoint from  $QR$ .

Suppose we flip a biased coin with  $P(\text{Heads}) = 3/4$  twice. What is the probability the second flip is Heads, given that at least one of the flips is Tails?

- (a)  $3/7$
- (b)  $4/7$
- (c)  $1/7$
- (d)  $3/4$
- (e)  $1/4$
- (f)  $9/16$
- (g)  $7/16$
- (h)  $1/3$
- (i)  $1/2$
- (j)  $1$
- (k)  $0$
- (l) None of these



Suppose we flip a biased coin with  $P(\text{Heads}) = 2/5$  twice. What is the probability the second flip is Heads, given that at least one of the flips is Tails?

- (a)  $2/7$
- (b)  $5/7$
- (c)  $1/7$
- (d)  $2/5$
- (e)  $3/5$
- (f)  $4/25$
- (g)  $21/25$
- (h)  $1/3$
- (i)  $1/2$
- (j)  $1$
- (k)  $0$
- (l) None of these

Suppose we flip a biased coin with  $P(\text{Heads}) = 4/5$  twice. What is the probability the second flip is Heads, given that at least one of the flips is Tails?

- (a)  $4/9$
- (b)  $5/9$
- (c)  $1/9$
- (d)  $4/5$
- (e)  $1/5$
- (f)  $16/25$
- (g)  $9/25$
- (h)  $1/3$
- (i)  $1/2$
- (j)  $1$
- (k)  $0$
- (l) None of these

Suppose we flip a biased coin with  $P(\text{Heads}) = 5/6$  twice. What is the probability the second flip is Heads, given that at least one of the flips is Tails?

- (a)  $5/11$
- (b)  $6/11$
- (c)  $1/11$
- (d)  $5/6$
- (e)  $1/6$
- (f)  $25/36$
- (g)  $11/36$
- (h)  $1/3$
- (i)  $1/2$
- (j)  $1$
- (k)  $0$
- (l) None of these

**Solution:** Let  $E$  be the event the first flip is heads and let  $F$  be the event the second flip is Heads. Then,

$$\begin{aligned}
 P(F|(EF)^c) &= \frac{P(F(EF)^c)}{P((EF)^c)} \\
 &= \frac{P(F(E^c \cup F^c))}{1 - P(EF)} \\
 &= \frac{P(FE^c)}{1 - q^2} \\
 &= \frac{q(1 - q)}{1 - q^2} \\
 &= \frac{q}{1 + q}
 \end{aligned}$$

If  $q = k/n$ , then  $P(F|(EF)^c) = \frac{k/n}{1+(k/n)} = \frac{k}{k+n}$ .